R1cs.v
@@ -1,22 +1,23 @@
 Require Import Metalib.Metatheory.
-From STLCZK Require Import Stlc.
+From STLCZK Require Import Gadgets.
 
 Require Import Coqprime.elliptic.ZEll.
 Require Import Coq.Numbers.BinNums.
 Require Export FMapAVL.
 Require Export Coq.Structures.OrderedTypeEx.
 
-Module M := FMapAVL.Make(Nat_as_OT).
-
-Module R1CS.
-  Import Stlc_Fp.
 
 
+Module QAP.
+  Include Gadgets.
+  Module M := FMapAVL.Make(Nat_as_OT).  
   (** Maps *)
   Definition NMap: Type -> Type := M.t.
   Definition find k (m: NMap Fp) := M.find k m.
   Definition update (p: nat * Fp) (m: NMap Fp) :=
-    M.add (fst p) (snd p) m.
+    match p with
+    | (f, s) => M.add f s m
+    end.
 
   Notation "k |-> v" := (pair k v) (at level 60).
   Notation "[ ]" := (M.empty Fp).
@@ -40,6 +41,13 @@ Module R1CS.
 
   Definition R1cs := list BilinearConstraint.
 
+  Inductive Circuit :=
+  | Add (a: Circuit) (b: Circuit)
+  | Mul (a: Circuit) (b: Circuit)
+  | In (index: nat)
+  | Witness (index: nat)
+  | Const (f: Fp).
+  
   (** Evaluate LC like this: const + (sum . map (+) $ vars) == 0 *)
   Definition evalLc(ctx: NMap Fp)(lc: Lc): option Fp :=
     M.fold
@@ -64,7 +72,7 @@ Module R1CS.
     evalBilinearConstraint ctx bc = Some fp_zero.
 
   Check checkBilinearConstraint.
-  Definition checkR1cs(ctx: NMap Fp)(r1cs: R1cs) := Forall (checkBilinearConstraint ctx) r1cs.
+  Definition checkR1cs(ctx: NMap Fp)(r1cs: R1cs) : Prop := Forall (checkBilinearConstraint ctx) r1cs.
 
   (** Helper monadic notation on options *)
   Notation "'return' e" := (Some e) (right associativity, at level 49).
@@ -75,29 +83,66 @@ Module R1CS.
         end)
          (right associativity, p pattern, at level 60, e1 at next level).
 
-  Inductive first_order: typ -> Prop :=
-  | fo_field: first_order ty_field
-  | fo_bool: first_order ty_bool.
-  
+ 
+End QAP.
+
+Require Import ExtLib.Data.Monads.StateMonad.
+Require Import ExtLib.Structures.Monads.
+
+(**
+   1. Use a state monad to compile equations to R1CS
+   2. R1CS semantics: 
+        For some z = vars ++ [1] ++ inputs, <A*z, B*z> = C*z
+   3. Use https://apps.cs.utexas.edu/tech_reports/reports/tr/TR-2112.pdf
+      for compilation
+   4. Prove each rewrite rule according to circuit_equiv.
+   5. Given rules: { 
+              proof1: tm_eq ~ eq_check,
+              proof2: tm_div ~ div_check,
+              proof3: tm_ifthenelse ~ ite_check,
+              ...
+            }
+      And (e: exp) -> e_check: R1CS and proof proof_e: e ~ e_check.
+*) 
+Module R1CS.
+  Include Gadgets.
+  Module Pair_Nats_OT := PairOrderedType Nat_as_OT Nat_as_OT.
+  Module M := FMapAVL.Make(Pair_Nats_OT).
+
+  (** Maps *)
+  Definition PMap: Type -> Type := M.t.
+  Definition find k (m: PMap Fp) := M.find k m.
+  Definition update (p: nat * nat * Fp) (m: PMap Fp) :=
+    match p with
+    | (a, b, v) => M.add (a, b) m
+    end.
+
+  Notation "k |-> v" := (pair k v) (at level 60).
+  Notation "[ ]" := (M.empty Fp).
+  Notation "[ p1 , .. , pn ]" := (update p1 .. (update pn (M.empty Fp)) .. ).
+
+  Record Constraints{F: Type} (f: F) :=
+    mkConstraints {
+        num_witness: nat;
+        num_inputs: nat;
+        num_constraints: nat;
+        A: PMap F; (** (num constraint, index of term i) -> Fp *)
+        B: PMap F;
+        C: PMap F
+      }.
+
+  Definition Constraint := state (Constraints Fp).
+
+  Set Typeclasses Debug. 
+  Definition witness: Constraint nat :=
+    bind get (fun x => num_witness).
+    
   (** 1. We have STLC term m: [] |- m: t -> t
       2. We need R1cs r, checkR1cs r
       3. We have term m, 
          eval ctx_inp m = (r, ctx')
    *)
   (** Compilation = solving *)
-
-  Fixpoint interp(ctx: NMap Fp)(e: exp) (normalizes: e -->* <{ fp v }>): option (Ctx * r1cs) :=
-    match e with
-    | tm_var_b n => (ctx, [])
-    | tm_var_f x => (ctx, [])
-    | tm_abs T e =>
-      (ctx2, p) <- compile ctx e (lc_trans lc) ;;
-      return (ctx2, p)
-    | tm_app e1 e2 =>
-      (ctx2, p1) <- compile ctx e
-      
-    | tm_let e1 e2 =>
-    | tm_binop a op_div b => 
-    | tm_constant c => (ctx, 
-
+  
+  
 End R1CS.
